some progress in teh soundness of memory solver/updater

memory_ops_solvers_impl.v
@@ -52,9 +52,9 @@ Module MemoryOpsSolversImpl.
   
   (* [soffset,soffset+size] does not overlap with [soffset',soffset'+size'] --- closed intervals *)
   (* We will mainly use it with size=31 or size=0 *)
-  Definition memory_slots_do_not_overlap (soffset soffset': sstack_val) (size size':N): bool :=
-    match soffset, soffset' with
-    | Val v1, Val v2 =>
+  Definition memory_slots_do_not_overlap (soffset soffset': sstack_val) (size size':N) (maxidx: nat) (sb: sbindings) (instk_height: nat) (ops: stack_op_instr_map): bool :=
+    match follow_in_smap soffset maxidx sb, follow_in_smap soffset' maxidx sb with
+    | Some (FollowSmapVal (SymBasicVal (Val v1)) _ _), Some (FollowSmapVal (SymBasicVal (Val v2)) _ _) => 
         let addr := (wordToN v1) in
         let addr' := (wordToN v2) in
         orb (addr+size <? addr')%N (addr'+size' <? addr)%N
@@ -69,21 +69,21 @@ Module MemoryOpsSolversImpl.
         if sstack_val_cmp (S (get_maxidx_smap m)) soffset soffset' (get_maxidx_smap m) (get_bindings_smap m) (get_maxidx_smap m) (get_bindings_smap m) instk_height ops then
           SymBasicVal svalue
         else
-          if memory_slots_do_not_overlap soffset soffset' 31 31 then
+          if memory_slots_do_not_overlap soffset soffset' 31 31 (get_maxidx_smap m) (get_bindings_smap m) instk_height ops then
             basic_mload_solver sstack_val_cmp soffset smem' instk_height m ops
           else
             SymMLOAD soffset smem
     | (U_MSTORE8 _ soffset' svalue)::smem' =>
-        if memory_slots_do_not_overlap soffset soffset' 31 0 then
+        if memory_slots_do_not_overlap soffset soffset' 31 0 (get_maxidx_smap m) (get_bindings_smap m) instk_height ops then
           basic_mload_solver sstack_val_cmp soffset smem' instk_height m ops
         else
           SymMLOAD soffset smem             
     end.
 
   (* mstore8 soffset_mstore8 is includes in soffset_mstore *)
-  Definition mstore8_is_included_in_mstore (soffset_mstore8 soffset_mstore: sstack_val) : bool :=
-    match soffset_mstore8, soffset_mstore with
-    | Val v1, Val v2 =>
+  Definition mstore8_is_included_in_mstore (soffset_mstore8 soffset_mstore: sstack_val) (maxidx: nat) (sb: sbindings) (instk_height: nat) (ops: stack_op_instr_map): bool :=
+    match follow_in_smap soffset_mstore8 maxidx sb, follow_in_smap soffset_mstore maxidx sb with
+    | Some (FollowSmapVal (SymBasicVal (Val v1)) _ _), Some (FollowSmapVal (SymBasicVal (Val v2)) _ _) => 
         let addr_mstore8 := (wordToN v1) in
         let addr_mstore := (wordToN v2) in
         andb (addr_mstore <=? addr_mstore8 )%N (addr_mstore8 <=? addr_mstore+31)%N
@@ -99,7 +99,7 @@ Module MemoryOpsSolversImpl.
         else
           (U_MSTORE sstack_val soffset' svalue)::(basic_smemory_updater_remove_mstore_dups sstack_val_cmp soffset_mstore smem' instk_height m ops)
     | (U_MSTORE8 _ soffset' svalue)::smem' =>
-        if mstore8_is_included_in_mstore soffset' soffset_mstore then
+        if mstore8_is_included_in_mstore soffset' soffset_mstore (get_maxidx_smap m) (get_bindings_smap m) instk_height ops then
           basic_smemory_updater_remove_mstore_dups sstack_val_cmp soffset_mstore smem' instk_height m ops (* we can also stop, since we will have at most one duplicate *)
         else
           (U_MSTORE8 sstack_val soffset' svalue)::(basic_smemory_updater_remove_mstore_dups sstack_val_cmp soffset_mstore smem' instk_height m ops)
