memory_ops_solvers_impl_soundness.v
@@ -1,7 +1,7 @@
 Require Import Arith.  
 Require Import Nat. 
 Require Import Bool.
-Require Import bbv.Word.
+Require Import bbv.Word. 
 Require Import Coq.NArith.NArith.
 Require Import List.
 Import ListNotations.
@@ -107,7 +107,7 @@ Module MemoryOpsSolversImplSoundness.
       unfold trivial_smemory_updater in H_updater.
       rewrite <- H_updater.
       intros stk mem strg ctx H_len_stk.
-      pose proof (valid_smemeory_when_extended_with_valid_update instk_height (get_maxidx_smap m) u smem H_valid_u H_valid_smem) as H_valid_u_smem.
+      pose proof (valid_smemory_when_extended_with_valid_update instk_height (get_maxidx_smap m) u smem H_valid_u H_valid_smem) as H_valid_u_smem.
       unfold valid_smap in H_valid_smap.
       symmetry in H_len_stk.
       pose proof (eval_smemory_succ instk_height (get_maxidx_smap m) (get_bindings_smap m) stk mem strg ctx ops (u::smem) H_len_stk H_valid_u_smem H_valid_smap) as H_eval_smemory_u_smem.
@@ -122,7 +122,7 @@ Lemma  H_memory_slots_do_not_overlap:
       valid_bindings instk_height maxidx sbindings ops ->
       valid_sstack_value instk_height maxidx soffset  ->
       valid_sstack_value instk_height maxidx soffset' ->
-      memory_slots_do_not_overlap soffset soffset' size size' = true ->
+      memory_slots_do_not_overlap soffset soffset' size size' maxidx sbindings instk_height ops = true ->
       forall stk mem strg ctx,
         (length stk) = instk_height ->
         exists v1 v2,
@@ -132,33 +132,68 @@ Lemma  H_memory_slots_do_not_overlap:
   Proof.
     intros soffset soffset' size size' maxidx sbindings instk_height ops.
     intros H_valid_sbindings H_valid_offset H_valid_offset' H_addr_nover.
-    intros stk mem strg ctx H_stk_len.
-
-    pose proof (eval_sstack_val'_succ (S maxidx) instk_height soffset stk mem strg ctx maxidx sbindings ops (eq_sym H_stk_len) H_valid_offset H_valid_sbindings (gt_Sn_n maxidx)) as H_eval_soffset.
-    pose proof (eval_sstack_val'_succ (S maxidx) instk_height soffset' stk mem strg ctx maxidx sbindings ops (eq_sym H_stk_len) H_valid_offset' H_valid_sbindings (gt_Sn_n maxidx)) as H_eval_soffset'.
-    destruct H_eval_soffset as [soffset_v H_eval_soffset].
-    destruct H_eval_soffset' as [soffset'_v H_eval_soffset'].
-
-    exists soffset_v.
-    exists soffset'_v.
-    repeat split. apply H_eval_soffset. apply H_eval_soffset'.
     unfold memory_slots_do_not_overlap in H_addr_nover.
-
-    destruct soffset; try discriminate.
-    destruct soffset'; try discriminate.
-
-    pose proof (eval_sstack_val'_Val val stk mem strg ctx maxidx sbindings ops) as H_eval_soffset_val.
-    rewrite H_eval_soffset_val in H_eval_soffset.
-    injection H_eval_soffset as H_eval_soffset.
     
-    pose proof (eval_sstack_val'_Val val0 stk mem strg ctx maxidx sbindings ops) as H_eval_soffset'_val.
-    rewrite H_eval_soffset'_val in H_eval_soffset'.
-    injection H_eval_soffset' as H_eval_soffset'.
+    destruct (follow_in_smap soffset maxidx sbindings) as [soffset_m|] eqn:E_follow_soffset; try discriminate.
+    destruct soffset_m; try discriminate.
+    destruct smv; try discriminate.
+    destruct val; try discriminate.
 
-    rewrite <- H_eval_soffset.
-    rewrite <- H_eval_soffset'.
-    
+    destruct (follow_in_smap soffset' maxidx sbindings) as [soffset'_m|] eqn:E_follow_soffset'; try discriminate.
+    destruct soffset'_m; try discriminate.
+    destruct smv; try discriminate.
+    destruct val0; try discriminate.
+
+    intros stk mem strg ctx.
+    intros H_stk_len.
+    unfold eval_sstack_val' at 1.
+    rewrite E_follow_soffset.
+    unfold eval_sstack_val' at 1.
+    rewrite E_follow_soffset'.
+    exists val.
+    exists val0.
+    split; try split; try reflexivity.
     apply H_addr_nover.
+  Qed.
+
+
+  Lemma  H_mstore8_is_included_in_mstore:
+    forall soffset_mstore8 soffset_mstore maxidx sbindings instk_height ops,
+      valid_bindings instk_height maxidx sbindings ops ->
+      valid_sstack_value instk_height maxidx soffset_mstore8  ->
+      valid_sstack_value instk_height maxidx soffset_mstore ->
+      mstore8_is_included_in_mstore soffset_mstore8 soffset_mstore maxidx sbindings instk_height ops = true ->
+      forall stk mem strg ctx,
+        (length stk) = instk_height ->
+        exists v1 v2,
+        eval_sstack_val' (S maxidx) soffset_mstore8 stk mem strg ctx maxidx sbindings ops = Some v1 /\
+          eval_sstack_val' (S maxidx) soffset_mstore stk mem strg ctx maxidx sbindings ops = Some v2 /\
+          andb ((wordToN v2) <=? (wordToN v1) )%N ((wordToN v1) <=? (wordToN v2)+31)%N = true.
+  Proof.
+    intros soffset_mstore8 soffset_mstore maxidx sbindings instk_height ops.
+    intros H_valid_sbindings H_valid_offset_mstore8 H_valid_offset_mstore H_addr_not_inc.
+    unfold mstore8_is_included_in_mstore in H_addr_not_inc.
+
+    destruct (follow_in_smap soffset_mstore8 maxidx sbindings) as [soffset_mstore8_m|] eqn:E_follow_soffset_mstore8; try discriminate.
+    destruct soffset_mstore8_m; try discriminate.
+    destruct smv; try discriminate.
+    destruct val; try discriminate.
+
+    destruct (follow_in_smap soffset_mstore maxidx sbindings) as [soffset_mstore_m|] eqn:E_follow_soffset_mstore; try discriminate.
+    destruct soffset_mstore_m; try discriminate.
+    destruct smv; try discriminate.
+    destruct val0; try discriminate.
+
+    intros stk mem strg ctx.
+    intros H_stk_len.
+    unfold eval_sstack_val' at 1.
+    rewrite E_follow_soffset_mstore8.
+    unfold eval_sstack_val' at 1.
+    rewrite E_follow_soffset_mstore.
+    exists val.
+    exists val0.
+    split; try split; try reflexivity.
+    apply H_addr_not_inc.
   Qed.
 
   Lemma basic_mload_solver_valid:
@@ -288,7 +323,72 @@ Proof.
   Admitted.
 
 
+Lemma two_consecutive_updates_same_address:
+  forall soffset soffset' svalue svalue' smem maxidx bs stk mem strg ctx ops v,
+    eval_sstack_val soffset stk mem strg ctx maxidx bs ops = Some v ->
+    eval_sstack_val soffset' stk mem strg ctx maxidx bs ops = Some v ->
+    eval_smemory (U_MSTORE sstack_val soffset svalue :: U_MSTORE sstack_val soffset' svalue' :: smem) maxidx bs stk mem strg ctx ops =
+      eval_smemory (U_MSTORE sstack_val soffset svalue :: smem) maxidx bs stk mem strg ctx ops.
+Proof.
+Admitted.
 
+Lemma two_consecutive_mstore8_updates_same_address:
+  forall soffset soffset' svalue svalue' smem maxidx bs stk mem strg ctx ops v,
+    eval_sstack_val soffset stk mem strg ctx maxidx bs ops = Some v ->
+    eval_sstack_val soffset' stk mem strg ctx maxidx bs ops = Some v ->
+    eval_smemory (U_MSTORE8 sstack_val soffset svalue :: U_MSTORE8 sstack_val soffset' svalue' :: smem) maxidx bs stk mem strg ctx ops =
+      eval_smemory (U_MSTORE8 sstack_val soffset svalue :: smem) maxidx bs stk mem strg ctx ops.
+Proof.
+Admitted.
+
+Lemma two_consecutive_updates_same_address_mstore8:
+  forall soffset_mstore8 soffset_mstore svalue8 svalue smem maxidx bs stk mem strg ctx ops v1 v2,
+    eval_sstack_val soffset_mstore8 stk mem strg ctx maxidx bs ops = Some v1 ->
+    eval_sstack_val soffset_mstore stk mem strg ctx maxidx bs ops = Some v2 ->
+    andb ((wordToN v2) <=? (wordToN v1) )%N ((wordToN v1) <=? (wordToN v2)+31)%N = true ->
+    eval_smemory (U_MSTORE sstack_val soffset_mstore svalue :: U_MSTORE8 sstack_val soffset_mstore8 svalue8 :: smem) maxidx bs stk mem strg ctx ops =
+      eval_smemory (U_MSTORE sstack_val soffset_mstore svalue :: smem) maxidx bs stk mem strg ctx ops.
+Proof.
+Admitted.
+
+Lemma mem_eq_when_after_update_eq:
+  forall mem1 mem2 u,
+    eval_common.EvalCommon.update_memory' mem1 u = eval_common.EvalCommon.update_memory' mem2 u ->
+    mem1 = mem2.
+Admitted.
+                                                                                                         
+Lemma N_of_nat_Sn:
+  forall x n, (x + N.of_nat (S n) = x+ 1 + N.of_nat n)%N.
+Proof.
+  intros x n.
+  apply N2Nat.inj_iff.
+  repeat rewrite N2Nat.inj_add.
+  intuition.
+Qed.
+
+
+Lemma mstore'_not_touched_addresses_remain_the_same:
+  forall sz mem w offset mem',
+    concrete_interpreter.ConcreteInterpreter.mstore' mem  (w : (word (sz*8))) offset = mem' ->
+    forall offset', (offset' >= offset + (N.of_nat sz))%N -> mem offset' = mem' offset'.
+Proof.
+  induction sz as [| sz' IHsz'].
+  + intros mem w n mem' H_mstore' n' H_n'_gt_n.
+    unfold concrete_interpreter.ConcreteInterpreter.mstore' in H_mstore'.
+    rewrite H_mstore'.
+    reflexivity.
+  + intros mem w offset mem' H_mstore' offset' H_n'_gt_n.
+    simpl in H_mstore'.
+    rewrite N_of_nat_Sn in H_n'_gt_n.
+    pose proof (IHsz' (fun offset' : N => if (offset' =? offset)%N then concrete_interpreter.ConcreteInterpreter.split1_byte w else mem offset')
+                     (concrete_interpreter.ConcreteInterpreter.split2_byte w) (offset+1)%N mem' H_mstore' offset' H_n'_gt_n) as IHsz'_0.
+    simpl in IHsz'_0.
+    destruct ((offset' =? offset)%N) eqn:E_offset_eq_offset'.
+    ++  apply N.eqb_eq in E_offset_eq_offset'.
+        intuition.        
+    ++ rewrite IHsz'_0.
+       reflexivity.
+Qed.
 
 Lemma basic_mload_solver_snd: mload_solver_ext_snd basic_mload_solver.
   unfold mload_solver_ext_snd.
@@ -765,8 +865,658 @@ Qed.
    Qed. 
 
 
+  
+  Lemma basic_smemory_updater_remove_dups_correct_eq_key:
+    forall sstack_val_cmp soffset svalue instk_height stk mem strg ctx m ops smem1 smem2 mem1 mem2 v,
+      symbolic_state_cmp.SymbolicStateCmp.safe_sstack_val_cmp_ext_1 sstack_val_cmp ->
+      length stk = instk_height ->
+      valid_sstack_value instk_height (get_maxidx_smap m) soffset ->
+      valid_sstack_value instk_height (get_maxidx_smap m) svalue ->
+      valid_smap instk_height (get_maxidx_smap m) (get_bindings_smap m) ops ->
+      valid_smemory instk_height (get_maxidx_smap m) smem1 ->
+      valid_smemory instk_height (get_maxidx_smap m) smem2 ->
+      eval_smemory (U_MSTORE sstack_val soffset svalue :: smem1) (get_maxidx_smap m) (get_bindings_smap m) stk mem strg ctx ops = Some mem1 ->
+      eval_smemory (U_MSTORE sstack_val soffset svalue :: smem2) (get_maxidx_smap m) (get_bindings_smap m) stk mem strg ctx ops = Some mem2 ->
+      eval_sstack_val' (S (get_maxidx_smap m)) soffset stk mem strg ctx (get_maxidx_smap m)  (get_bindings_smap m) ops = Some v ->
+      concrete_interpreter.ConcreteInterpreter.mload mem1 v = concrete_interpreter.ConcreteInterpreter.mload mem2 v.
+  Proof.
+    intros sstack_val_cmp soffset svalue instk_height stk mem strg ctx m ops smem1 smem2 mem1 mem2 v.
+    intros H_sstack_val_cmp_snd H_stk_len H_valid_soffset H_valid_svalue H_valid_smap H_valid_smem1 H_valid_smem2 H_eval_smem1 H_eval_smem2 H_eval_soffset.
+
+    unfold eval_smemory in H_eval_smem1.
+    destruct (map_option (eval_common.EvalCommon.instantiate_memory_update (fun sv : sstack_val => eval_sstack_val sv stk mem strg ctx (get_maxidx_smap m) (get_bindings_smap m) ops)) (U_MSTORE sstack_val soffset svalue :: smem1)) as [updates1|] eqn:E_mo_1; try discriminate.
+    injection H_eval_smem1 as H_mem1.
+
+    unfold eval_smemory in H_eval_smem2.
+    destruct (map_option (eval_common.EvalCommon.instantiate_memory_update (fun sv : sstack_val => eval_sstack_val sv stk mem strg ctx (get_maxidx_smap m) (get_bindings_smap m) ops)) (U_MSTORE sstack_val soffset svalue :: smem2)) as [updates2|] eqn:E_mo_2; try discriminate.
+    injection H_eval_smem2 as H_mem2.
+    
+
+    pose proof (map_option_split (memory_update sstack_val) (memory_update EVMWord) (eval_common.EvalCommon.instantiate_memory_update (fun sv : sstack_val => eval_sstack_val sv stk mem strg ctx (get_maxidx_smap m) (get_bindings_smap m) ops)) smem1 updates1 (U_MSTORE sstack_val soffset svalue) E_mo_1) as E_mo_1_0.
+    destruct E_mo_1_0 as [e1 [updates1' [E_updates1 [E_e1 H_mo_1_0]]]].
+
+    pose proof (map_option_split (memory_update sstack_val) (memory_update EVMWord) (eval_common.EvalCommon.instantiate_memory_update (fun sv : sstack_val => eval_sstack_val sv stk mem strg ctx (get_maxidx_smap m) (get_bindings_smap m) ops)) smem2 updates2 (U_MSTORE sstack_val soffset svalue) E_mo_2) as E_mo_2_0.
+    destruct E_mo_2_0 as [e2 [updates2' [E_updates2 [E_e2 H_mo_2_0]]]].
+
+
+    unfold eval_common.EvalCommon.instantiate_memory_update in E_e1.
+    unfold eval_sstack_val in E_e1.
+    rewrite H_eval_soffset in E_e1.
+    destruct (eval_sstack_val' (S (get_maxidx_smap m)) svalue stk mem strg ctx (get_maxidx_smap m) (get_bindings_smap m) ops) as [svalue_v|] eqn:H_eval_svalue; try discriminate.
+    injection E_e1 as E_e1.
+    
+    unfold eval_common.EvalCommon.instantiate_memory_update in E_e2.
+    unfold eval_sstack_val in E_e2.
+    rewrite H_eval_soffset in E_e2.
+    rewrite H_eval_svalue in E_e2.
+    injection E_e2 as E_e2.
+    
+    rewrite <- H_mem1.
+    rewrite <- H_mem2.
+    rewrite E_updates1.
+    rewrite E_updates2.
+    rewrite <- E_e1.
+    rewrite <- E_e2.
+
+    unfold eval_common.EvalCommon.update_memory.
+    fold eval_common.EvalCommon.update_memory.
+    unfold eval_common.EvalCommon.update_memory'.
+    
+    repeat rewrite mload_mstore_same_address.
+    reflexivity.
+  Qed.
+    
+  
+    Lemma basic_smemory_updater_remove_mstore_dups_correct:
+    forall sstack_val_cmp soffset svalue instk_height stk mem strg ctx m ops,
+      symbolic_state_cmp.SymbolicStateCmp.safe_sstack_val_cmp_ext_1 sstack_val_cmp ->
+      length stk = instk_height ->
+      valid_sstack_value instk_height (get_maxidx_smap m) soffset ->
+      valid_sstack_value instk_height (get_maxidx_smap m) svalue ->
+      valid_smap instk_height (get_maxidx_smap m) (get_bindings_smap m) ops ->
+      forall smem smem_r,
+      valid_smemory instk_height (get_maxidx_smap m) smem ->
+      basic_smemory_updater_remove_mstore_dups sstack_val_cmp soffset smem instk_height m ops = smem_r ->
+      exists mem1 mem2,
+        eval_smemory (U_MSTORE sstack_val soffset svalue :: smem) (get_maxidx_smap m) (get_bindings_smap m) stk mem strg ctx ops =
+          Some mem1 /\
+          eval_smemory (U_MSTORE sstack_val soffset svalue :: smem_r) (get_maxidx_smap m) (get_bindings_smap m) stk mem strg ctx ops = Some mem2 /\
+          forall w, mem1 w = mem2 w.
+    Proof.
+      intros sstack_val_cmp soffset svalue instk_height stk mem strg ctx m ops.
+      intros H_sstack_val_cmp_snd H_stk_len H_valid_soffset H_valid_svalue H_valid_smap.
+ 
+      induction smem as [|u smem' IHsmem'].
+      + intros smem_r H_valid_smem H_basic_mstore_up.
+        simpl in H_basic_mstore_up.
+        rewrite <- H_basic_mstore_up.
+        assert(H_valid_u: valid_smemory instk_height (get_maxidx_smap m)  [U_MSTORE sstack_val soffset svalue]). simpl. auto.
+        pose proof (eval_smemory_succ instk_height (get_maxidx_smap m) (get_bindings_smap m) stk mem strg ctx ops [U_MSTORE sstack_val soffset svalue] (eq_sym H_stk_len) H_valid_u H_valid_smap) as H_eval_u.
+        destruct H_eval_u as [smem' H_eval_u].
+        rewrite H_eval_u.
+        exists smem'.
+        exists smem'.
+        auto.
+      + intros smem_r H_valid_smem H_basic_mstore_up.
+        simpl in H_basic_mstore_up.
+        destruct u as [soffset' svalue'|soffset' svalue'] eqn:E_u.
+        (* MSTORE *)
+        ++ simpl in H_valid_smem.
+           destruct H_valid_smem as [ [H_valid_soffset' H_valid_svalue'] H_valid_smem'].
+           destruct (sstack_val_cmp (S (get_maxidx_smap m)) soffset soffset' (get_maxidx_smap m) (get_bindings_smap m) (get_maxidx_smap m) (get_bindings_smap m) instk_height ops) eqn:E_cmp_soffset_soffset'.
+           +++ pose proof (IHsmem' smem_r H_valid_smem' H_basic_mstore_up) as IHsmem'_0.       
+               destruct IHsmem'_0 as [mem1' [mem2' [IHsmem'_0_1 [IHsmem'_0_2 IHsmem'_0_3]]]].
+               unfold safe_sstack_val_cmp_ext_1_d in H_sstack_val_cmp_snd.
+               unfold safe_sstack_val_cmp in H_sstack_val_cmp_snd.
+               pose proof (H_sstack_val_cmp_snd (S (get_maxidx_smap m)) (S (get_maxidx_smap m)) (Nat.le_refl (S (get_maxidx_smap m))) soffset soffset' (get_maxidx_smap m) (get_bindings_smap m) (get_maxidx_smap m) (get_bindings_smap m) instk_height ops H_valid_soffset H_valid_soffset' H_valid_smap H_valid_smap E_cmp_soffset_soffset' stk mem strg ctx H_stk_len) as H_eq_soffset_soffset'.
+               destruct H_eq_soffset_soffset' as [soffset_v [ H_eval_soffset H_eval_soffset']].
+
+               pose proof (two_consecutive_updates_same_address soffset soffset' svalue svalue' smem' (get_maxidx_smap m) (get_bindings_smap m) stk mem strg ctx ops soffset_v H_eval_soffset H_eval_soffset') as H_remove_soffset'.
+               rewrite H_remove_soffset'.
+
+               rewrite IHsmem'_0_1.
+               rewrite IHsmem'_0_2.
+
+               exists mem1'.
+               exists mem2'.
+               
+               repeat split; try reflexivity.
+               apply IHsmem'_0_3.
+           +++ rewrite <- H_basic_mstore_up. 
+
+               remember (basic_smemory_updater_remove_mstore_dups sstack_val_cmp soffset smem' instk_height m ops) as smem'_r.
+               rewrite Heqsmem'_r in *.
+               symmetry in Heqsmem'_r.
+               rewrite Heqsmem'_r.
+               
+               pose proof (IHsmem' smem'_r H_valid_smem' Heqsmem'_r) as IHsmem'_0.
+               destruct IHsmem'_0 as [mem1' [mem2' [H_eval_u_smem' [H_eval_u_smem'_r H_eq_mem1'_mem2']]]].
+               apply functional_extensionality in H_eq_mem1'_mem2' as H_eq_mem1'_mem2'_f.
+
+               pose proof (eval_sstack_val'_succ (S (get_maxidx_smap m)) instk_height soffset stk mem strg ctx (get_maxidx_smap m) (get_bindings_smap m) ops (eq_sym H_stk_len) H_valid_soffset H_valid_smap (gt_Sn_n ((get_maxidx_smap m)))) as H_eval_soffset.
+               destruct H_eval_soffset as [soffset_v H_eval_soffset].
+               
+               pose proof (eval_sstack_val'_succ (S (get_maxidx_smap m)) instk_height soffset' stk mem strg ctx (get_maxidx_smap m) (get_bindings_smap m) ops (eq_sym H_stk_len) H_valid_soffset' H_valid_smap (gt_Sn_n ((get_maxidx_smap m)))) as H_eval_soffset'.
+               destruct H_eval_soffset' as [soffset'_v H_eval_soffset'].
+
+               pose proof (eval_sstack_val'_succ (S (get_maxidx_smap m)) instk_height svalue stk mem strg ctx (get_maxidx_smap m) (get_bindings_smap m) ops (eq_sym H_stk_len) H_valid_svalue H_valid_smap (gt_Sn_n ((get_maxidx_smap m)))) as H_eval_svalue.
+               destruct H_eval_svalue as [svlaue_v H_eval_svalue].
+
+               pose proof (eval_sstack_val'_succ (S (get_maxidx_smap m)) instk_height svalue' stk mem strg ctx (get_maxidx_smap m) (get_bindings_smap m) ops (eq_sym H_stk_len) H_valid_svalue' H_valid_smap (gt_Sn_n ((get_maxidx_smap m)))) as H_eval_svalue'.
+               destruct H_eval_svalue' as [svlaue_v' H_eval_svalue'].
+
+               unfold eval_smemory.
+               unfold map_option.
+               repeat rewrite <- map_option_ho.
+
+               unfold eval_common.EvalCommon.instantiate_memory_update at 1.
+               unfold eval_sstack_val.
+               rewrite H_eval_soffset.
+               rewrite H_eval_svalue.
+
+               unfold eval_common.EvalCommon.instantiate_memory_update at 1.
+               unfold eval_sstack_val.
+               rewrite H_eval_soffset'.
+               rewrite H_eval_svalue'.
+              
+               unfold eval_common.EvalCommon.instantiate_memory_update at 2.
+               rewrite H_eval_soffset.
+               rewrite H_eval_svalue.
+
+               unfold eval_common.EvalCommon.instantiate_memory_update at 2.
+               unfold eval_sstack_val.
+               rewrite H_eval_soffset'.
+               rewrite H_eval_svalue'.
+
+               unfold eval_smemory in H_eval_u_smem'.
+               unfold eval_sstack_val in  H_eval_u_smem'.
+               
+
+               destruct (map_option (eval_common.EvalCommon.instantiate_memory_update (fun sv : sstack_val => eval_sstack_val'  (S (get_maxidx_smap m)) sv stk mem strg ctx (get_maxidx_smap m) (get_bindings_smap m) ops)) (U_MSTORE sstack_val soffset svalue :: smem')) as [updates1|] eqn:E_mo_1; try discriminate.
+               pose proof (map_option_split (memory_update sstack_val) (memory_update EVMWord) (eval_common.EvalCommon.instantiate_memory_update (fun sv : sstack_val => eval_sstack_val' (S (get_maxidx_smap m)) sv stk mem strg ctx (get_maxidx_smap m) (get_bindings_smap m) ops)) smem' updates1 (U_MSTORE sstack_val soffset svalue) E_mo_1) as E_mo_1_split.
+               destruct E_mo_1_split as [e1 [smem'' [E_updates_1 [E_mo_1_0 E_mo_1_1]]]].
+               rewrite E_mo_1_1.
+
+               unfold eval_smemory in H_eval_u_smem'_r.
+               unfold eval_sstack_val in  H_eval_u_smem'_r.
+               destruct (map_option (eval_common.EvalCommon.instantiate_memory_update (fun sv : sstack_val => eval_sstack_val'  (S (get_maxidx_smap m)) sv stk mem strg ctx (get_maxidx_smap m) (get_bindings_smap m) ops)) (U_MSTORE sstack_val soffset svalue :: smem'_r)) as [updates2|] eqn:E_mo_2; try discriminate.
+               pose proof (map_option_split (memory_update sstack_val) (memory_update EVMWord) (eval_common.EvalCommon.instantiate_memory_update (fun sv : sstack_val => eval_sstack_val' (S (get_maxidx_smap m)) sv stk mem strg ctx (get_maxidx_smap m) (get_bindings_smap m) ops)) smem'_r updates2 (U_MSTORE sstack_val soffset svalue) E_mo_2) as E_mo_2_split.
+               destruct E_mo_2_split as [e2 [smem'_r' [E_updates_2 [E_mo_2_0 E_mo_2_1]]]].
+               rewrite E_mo_2_1.
+
+               exists (eval_common.EvalCommon.update_memory mem (U_MSTORE EVMWord soffset_v svlaue_v :: U_MSTORE EVMWord soffset'_v svlaue_v' :: smem'')).
+               exists (eval_common.EvalCommon.update_memory mem (U_MSTORE EVMWord soffset_v svlaue_v :: U_MSTORE EVMWord soffset'_v svlaue_v' :: smem'_r')).
+	       split. reflexivity.
+               split. reflexivity.
+               intro w.
+               
+               unfold eval_common.EvalCommon.update_memory.
+               fold eval_common.EvalCommon.update_memory.
+
+               unfold eval_common.EvalCommon.instantiate_memory_update in E_mo_1_0.
+               rewrite H_eval_soffset in E_mo_1_0.
+               rewrite H_eval_svalue in E_mo_1_0.
+               injection E_mo_1_0 as E_e1.
+               
+               unfold eval_common.EvalCommon.instantiate_memory_update in E_mo_2_0.
+               rewrite H_eval_soffset in E_mo_2_0.
+               rewrite H_eval_svalue in E_mo_2_0.
+               injection E_mo_2_0 as E_e2.
+
+               rewrite E_updates_1 in H_eval_u_smem'.
+               unfold eval_common.EvalCommon.update_memory in H_eval_u_smem'.
+               fold eval_common.EvalCommon.update_memory in H_eval_u_smem'.
+               injection H_eval_u_smem' as H_eval_u_smem'.
+
+               rewrite E_updates_2 in H_eval_u_smem'_r.
+               unfold eval_common.EvalCommon.update_memory in H_eval_u_smem'_r.
+               fold eval_common.EvalCommon.update_memory in H_eval_u_smem'_r.
+               injection H_eval_u_smem'_r as H_eval_u_smem'_r.
+               rewrite H_eq_mem1'_mem2'_f in H_eval_u_smem'.
+               rewrite <- H_eval_u_smem'_r in H_eval_u_smem'.
+
+               rewrite <- E_e1 in H_eval_u_smem'.
+               rewrite <- E_e2 in H_eval_u_smem'.
+
+               apply mem_eq_when_after_update_eq in H_eval_u_smem'.
+               rewrite H_eval_u_smem'.
+               reflexivity.
+
+        (* MSTOR8 *)
+        ++ simpl in H_valid_smem.
+           destruct H_valid_smem as [ [H_valid_soffset' H_valid_svalue'] H_valid_smem'].
+           destruct (mstore8_is_included_in_mstore soffset' soffset) eqn:E_mstore8_inc.
+           +++ pose proof (IHsmem' smem_r H_valid_smem' H_basic_mstore_up) as IHsmem'_0.
+               destruct IHsmem'_0 as [mem1' [mem2' [IHsmem'_0_1 [IHsmem'_0_2 IHsmem'_0_3]]]].
+
+
+               pose proof (H_mstore8_is_included_in_mstore soffset' soffset (get_maxidx_smap m) (get_bindings_smap m) instk_height ops H_valid_smap H_valid_soffset' H_valid_soffset E_mstore8_inc stk mem strg ctx H_stk_len) as E_mstore8_not_inc.
+               destruct E_mstore8_not_inc as [soffset'_v [soffset_v [H_eval_soffset' [H_eval_soffset H_addr_inc]]]].
+               
+               pose proof (two_consecutive_updates_same_address_mstore8 soffset' soffset svalue' svalue smem' (get_maxidx_smap m) (get_bindings_smap m) stk mem strg ctx ops soffset'_v soffset_v H_eval_soffset' H_eval_soffset H_addr_inc) as H_remove_soffset'.
+
+               rewrite H_remove_soffset'.
+
+               rewrite IHsmem'_0_1.
+               rewrite IHsmem'_0_2.
+
+               exists mem1'.
+               exists mem2'.
+               
+               repeat split; try reflexivity.
+               apply IHsmem'_0_3.
+
+           +++ rewrite <- H_basic_mstore_up. 
+
+               remember (basic_smemory_updater_remove_mstore_dups sstack_val_cmp soffset smem' instk_height m ops) as smem'_r.
+               rewrite Heqsmem'_r in *.
+               symmetry in Heqsmem'_r.
+               rewrite Heqsmem'_r.
+               
+               pose proof (IHsmem' smem'_r H_valid_smem' Heqsmem'_r) as IHsmem'_0.
+               destruct IHsmem'_0 as [mem1' [mem2' [H_eval_u_smem' [H_eval_u_smem'_r H_eq_mem1'_mem2']]]].
+               apply functional_extensionality in H_eq_mem1'_mem2' as H_eq_mem1'_mem2'_f.
+
+               pose proof (eval_sstack_val'_succ (S (get_maxidx_smap m)) instk_height soffset stk mem strg ctx (get_maxidx_smap m) (get_bindings_smap m) ops (eq_sym H_stk_len) H_valid_soffset H_valid_smap (gt_Sn_n ((get_maxidx_smap m)))) as H_eval_soffset.
+               destruct H_eval_soffset as [soffset_v H_eval_soffset].
+               
+               pose proof (eval_sstack_val'_succ (S (get_maxidx_smap m)) instk_height soffset' stk mem strg ctx (get_maxidx_smap m) (get_bindings_smap m) ops (eq_sym H_stk_len) H_valid_soffset' H_valid_smap (gt_Sn_n ((get_maxidx_smap m)))) as H_eval_soffset'.
+               destruct H_eval_soffset' as [soffset'_v H_eval_soffset'].
+
+               pose proof (eval_sstack_val'_succ (S (get_maxidx_smap m)) instk_height svalue stk mem strg ctx (get_maxidx_smap m) (get_bindings_smap m) ops (eq_sym H_stk_len) H_valid_svalue H_valid_smap (gt_Sn_n ((get_maxidx_smap m)))) as H_eval_svalue.
+               destruct H_eval_svalue as [svlaue_v H_eval_svalue].
+
+               pose proof (eval_sstack_val'_succ (S (get_maxidx_smap m)) instk_height svalue' stk mem strg ctx (get_maxidx_smap m) (get_bindings_smap m) ops (eq_sym H_stk_len) H_valid_svalue' H_valid_smap (gt_Sn_n ((get_maxidx_smap m)))) as H_eval_svalue'.
+               destruct H_eval_svalue' as [svlaue_v' H_eval_svalue'].
+
+               unfold eval_smemory.
+               unfold map_option.
+               repeat rewrite <- map_option_ho.
+
+               unfold eval_common.EvalCommon.instantiate_memory_update at 1.
+               unfold eval_sstack_val.
+               rewrite H_eval_soffset.
+               rewrite H_eval_svalue.
+
+               unfold eval_common.EvalCommon.instantiate_memory_update at 1.
+               unfold eval_sstack_val.
+               rewrite H_eval_soffset'.
+               rewrite H_eval_svalue'.
+              
+               unfold eval_common.EvalCommon.instantiate_memory_update at 2.
+               rewrite H_eval_soffset.
+               rewrite H_eval_svalue.
+
+               unfold eval_common.EvalCommon.instantiate_memory_update at 2.
+               unfold eval_sstack_val.
+               rewrite H_eval_soffset'.
+               rewrite H_eval_svalue'.
+
+               unfold eval_smemory in H_eval_u_smem'.
+               unfold eval_sstack_val in  H_eval_u_smem'.
+               
+
+               destruct (map_option (eval_common.EvalCommon.instantiate_memory_update (fun sv : sstack_val => eval_sstack_val'  (S (get_maxidx_smap m)) sv stk mem strg ctx (get_maxidx_smap m) (get_bindings_smap m) ops)) (U_MSTORE sstack_val soffset svalue :: smem')) as [updates1|] eqn:E_mo_1; try discriminate.
+               pose proof (map_option_split (memory_update sstack_val) (memory_update EVMWord) (eval_common.EvalCommon.instantiate_memory_update (fun sv : sstack_val => eval_sstack_val' (S (get_maxidx_smap m)) sv stk mem strg ctx (get_maxidx_smap m) (get_bindings_smap m) ops)) smem' updates1 (U_MSTORE sstack_val soffset svalue) E_mo_1) as E_mo_1_split.
+               destruct E_mo_1_split as [e1 [smem'' [E_updates_1 [E_mo_1_0 E_mo_1_1]]]].
+               rewrite E_mo_1_1.
+
+               unfold eval_smemory in H_eval_u_smem'_r.
+               unfold eval_sstack_val in  H_eval_u_smem'_r.
+               destruct (map_option (eval_common.EvalCommon.instantiate_memory_update (fun sv : sstack_val => eval_sstack_val'  (S (get_maxidx_smap m)) sv stk mem strg ctx (get_maxidx_smap m) (get_bindings_smap m) ops)) (U_MSTORE sstack_val soffset svalue :: smem'_r)) as [updates2|] eqn:E_mo_2; try discriminate.
+               pose proof (map_option_split (memory_update sstack_val) (memory_update EVMWord) (eval_common.EvalCommon.instantiate_memory_update (fun sv : sstack_val => eval_sstack_val' (S (get_maxidx_smap m)) sv stk mem strg ctx (get_maxidx_smap m) (get_bindings_smap m) ops)) smem'_r updates2 (U_MSTORE sstack_val soffset svalue) E_mo_2) as E_mo_2_split.
+               destruct E_mo_2_split as [e2 [smem'_r' [E_updates_2 [E_mo_2_0 E_mo_2_1]]]].
+               rewrite E_mo_2_1.
+
+               exists (eval_common.EvalCommon.update_memory mem (U_MSTORE EVMWord soffset_v svlaue_v :: U_MSTORE8 EVMWord soffset'_v svlaue_v' :: smem'')).
+               exists (eval_common.EvalCommon.update_memory mem (U_MSTORE EVMWord soffset_v svlaue_v :: U_MSTORE8 EVMWord soffset'_v svlaue_v' :: smem'_r')).
+	       split. reflexivity.
+               split. reflexivity.
+               intro w.
+               
+               unfold eval_common.EvalCommon.update_memory.
+               fold eval_common.EvalCommon.update_memory.
+
+               unfold eval_common.EvalCommon.instantiate_memory_update in E_mo_1_0.
+               rewrite H_eval_soffset in E_mo_1_0.
+               rewrite H_eval_svalue in E_mo_1_0.
+               injection E_mo_1_0 as E_e1.
+               
+               unfold eval_common.EvalCommon.instantiate_memory_update in E_mo_2_0.
+               rewrite H_eval_soffset in E_mo_2_0.
+               rewrite H_eval_svalue in E_mo_2_0.
+               injection E_mo_2_0 as E_e2.
+
+               rewrite E_updates_1 in H_eval_u_smem'.
+               unfold eval_common.EvalCommon.update_memory in H_eval_u_smem'.
+               fold eval_common.EvalCommon.update_memory in H_eval_u_smem'.
+               injection H_eval_u_smem' as H_eval_u_smem'.
+
+               rewrite E_updates_2 in H_eval_u_smem'_r.
+               unfold eval_common.EvalCommon.update_memory in H_eval_u_smem'_r.
+               fold eval_common.EvalCommon.update_memory in H_eval_u_smem'_r.
+               injection H_eval_u_smem'_r as H_eval_u_smem'_r.
+               rewrite H_eq_mem1'_mem2'_f in H_eval_u_smem'.
+               rewrite <- H_eval_u_smem'_r in H_eval_u_smem'.
+
+               rewrite <- E_e1 in H_eval_u_smem'.
+               rewrite <- E_e2 in H_eval_u_smem'.
+
+               apply mem_eq_when_after_update_eq in H_eval_u_smem'.
+               rewrite H_eval_u_smem'.
+               reflexivity.
+Qed.
+
+
+
+    Lemma basic_smemory_updater_remove_mstore8_dups_correct:
+      forall sstack_val_cmp soffset svalue instk_height stk mem strg ctx m ops,
+        symbolic_state_cmp.SymbolicStateCmp.safe_sstack_val_cmp_ext_1 sstack_val_cmp ->
+        length stk = instk_height ->
+        valid_sstack_value instk_height (get_maxidx_smap m) soffset ->
+        valid_sstack_value instk_height (get_maxidx_smap m) svalue ->
+        valid_smap instk_height (get_maxidx_smap m) (get_bindings_smap m) ops ->
+        forall smem smem',
+          valid_smemory instk_height (get_maxidx_smap m) smem ->
+          basic_smemory_updater_remove_mstore8_dups sstack_val_cmp soffset smem instk_height m ops = smem' ->
+          exists mem1 mem2,
+            eval_smemory (U_MSTORE8 sstack_val soffset svalue :: smem) (get_maxidx_smap m) (get_bindings_smap m) stk mem strg ctx ops =
+          Some mem1 /\
+              eval_smemory (U_MSTORE8 sstack_val soffset svalue :: smem') (get_maxidx_smap m) (get_bindings_smap m) stk mem strg ctx ops = Some mem2 /\
+              forall w, mem1 w = mem2 w.
+    Proof.
+      intros sstack_val_cmp soffset svalue instk_height stk mem strg ctx m ops.
+      intros H_sstack_val_cmp_snd H_stk_len H_valid_soffset H_valid_svalue H_valid_smap.
+ 
+      induction smem as [|u smem' IHsmem'].
+      + intros smem_r H_valid_smem H_basic_mstore_up.
+        simpl in H_basic_mstore_up.
+        rewrite <- H_basic_mstore_up.
+        assert(H_valid_u: valid_smemory instk_height (get_maxidx_smap m)  [U_MSTORE sstack_val soffset svalue]). simpl. auto.
+        pose proof (eval_smemory_succ instk_height (get_maxidx_smap m) (get_bindings_smap m) stk mem strg ctx ops [U_MSTORE8 sstack_val soffset svalue] (eq_sym H_stk_len) H_valid_u H_valid_smap) as H_eval_u.
+        destruct H_eval_u as [smem' H_eval_u].
+        rewrite H_eval_u.
+        exists smem'.
+        exists smem'.
+        auto.
+      + intros smem_r H_valid_smem H_basic_mstore_up.
+        simpl in H_basic_mstore_up.
+        destruct u as [soffset' svalue'|soffset' svalue'] eqn:E_u.
+        (* MSTORE *)
+        ++ simpl in H_valid_smem.
+           destruct H_valid_smem as [ [H_valid_soffset' H_valid_svalue'] H_valid_smem'].
+
+           rewrite <- H_basic_mstore_up. 
+
+           remember (basic_smemory_updater_remove_mstore8_dups sstack_val_cmp soffset smem' instk_height m ops) as smem'_r.
+           rewrite Heqsmem'_r in *.
+           symmetry in Heqsmem'_r.
+           rewrite Heqsmem'_r.
+               
+           pose proof (IHsmem' smem'_r H_valid_smem' Heqsmem'_r) as IHsmem'_0.
+           destruct IHsmem'_0 as [mem1' [mem2' [H_eval_u_smem' [H_eval_u_smem'_r H_eq_mem1'_mem2']]]].
+           apply functional_extensionality in H_eq_mem1'_mem2' as H_eq_mem1'_mem2'_f.
+           
+           pose proof (eval_sstack_val'_succ (S (get_maxidx_smap m)) instk_height soffset stk mem strg ctx (get_maxidx_smap m) (get_bindings_smap m) ops (eq_sym H_stk_len) H_valid_soffset H_valid_smap (gt_Sn_n ((get_maxidx_smap m)))) as H_eval_soffset.
+           destruct H_eval_soffset as [soffset_v H_eval_soffset].
+           
+           pose proof (eval_sstack_val'_succ (S (get_maxidx_smap m)) instk_height soffset' stk mem strg ctx (get_maxidx_smap m) (get_bindings_smap m) ops (eq_sym H_stk_len) H_valid_soffset' H_valid_smap (gt_Sn_n ((get_maxidx_smap m)))) as H_eval_soffset'.
+           destruct H_eval_soffset' as [soffset'_v H_eval_soffset'].
+           
+           pose proof (eval_sstack_val'_succ (S (get_maxidx_smap m)) instk_height svalue stk mem strg ctx (get_maxidx_smap m) (get_bindings_smap m) ops (eq_sym H_stk_len) H_valid_svalue H_valid_smap (gt_Sn_n ((get_maxidx_smap m)))) as H_eval_svalue.
+           destruct H_eval_svalue as [svlaue_v H_eval_svalue].
+           
+           pose proof (eval_sstack_val'_succ (S (get_maxidx_smap m)) instk_height svalue' stk mem strg ctx (get_maxidx_smap m) (get_bindings_smap m) ops (eq_sym H_stk_len) H_valid_svalue' H_valid_smap (gt_Sn_n ((get_maxidx_smap m)))) as H_eval_svalue'.
+           destruct H_eval_svalue' as [svlaue_v' H_eval_svalue'].
+           
+           unfold eval_smemory.
+           unfold map_option.
+           repeat rewrite <- map_option_ho.
+           
+           unfold eval_common.EvalCommon.instantiate_memory_update at 1.
+           unfold eval_sstack_val.
+           rewrite H_eval_soffset.
+           rewrite H_eval_svalue.
+           
+           unfold eval_common.EvalCommon.instantiate_memory_update at 1.
+           unfold eval_sstack_val.
+           rewrite H_eval_soffset'.
+           rewrite H_eval_svalue'.
+           
+           unfold eval_common.EvalCommon.instantiate_memory_update at 2.
+           rewrite H_eval_soffset.
+           rewrite H_eval_svalue.
+           
+           unfold eval_common.EvalCommon.instantiate_memory_update at 2.
+           unfold eval_sstack_val.
+           rewrite H_eval_soffset'.
+           rewrite H_eval_svalue'.
+           
+           unfold eval_smemory in H_eval_u_smem'.
+           unfold eval_sstack_val in  H_eval_u_smem'.
+           
+
+           destruct (map_option (eval_common.EvalCommon.instantiate_memory_update (fun sv : sstack_val => eval_sstack_val'  (S (get_maxidx_smap m)) sv stk mem strg ctx (get_maxidx_smap m) (get_bindings_smap m) ops)) (U_MSTORE8 sstack_val soffset svalue :: smem')) as [updates1|] eqn:E_mo_1; try discriminate.
+           pose proof (map_option_split (memory_update sstack_val) (memory_update EVMWord) (eval_common.EvalCommon.instantiate_memory_update (fun sv : sstack_val => eval_sstack_val' (S (get_maxidx_smap m)) sv stk mem strg ctx (get_maxidx_smap m) (get_bindings_smap m) ops)) smem' updates1 (U_MSTORE8 sstack_val soffset svalue) E_mo_1) as E_mo_1_split.
+           destruct E_mo_1_split as [e1 [smem'' [E_updates_1 [E_mo_1_0 E_mo_1_1]]]].
+           rewrite E_mo_1_1.
+
+           unfold eval_smemory in H_eval_u_smem'_r.
+           unfold eval_sstack_val in  H_eval_u_smem'_r.
+           destruct (map_option (eval_common.EvalCommon.instantiate_memory_update (fun sv : sstack_val => eval_sstack_val'  (S (get_maxidx_smap m)) sv stk mem strg ctx (get_maxidx_smap m) (get_bindings_smap m) ops)) (U_MSTORE8 sstack_val soffset svalue :: smem'_r)) as [updates2|] eqn:E_mo_2; try discriminate.
+           pose proof (map_option_split (memory_update sstack_val) (memory_update EVMWord) (eval_common.EvalCommon.instantiate_memory_update (fun sv : sstack_val => eval_sstack_val' (S (get_maxidx_smap m)) sv stk mem strg ctx (get_maxidx_smap m) (get_bindings_smap m) ops)) smem'_r updates2 (U_MSTORE8 sstack_val soffset svalue) E_mo_2) as E_mo_2_split.
+           destruct E_mo_2_split as [e2 [smem'_r' [E_updates_2 [E_mo_2_0 E_mo_2_1]]]].
+           rewrite E_mo_2_1.
+           
+           exists (eval_common.EvalCommon.update_memory mem (U_MSTORE8 EVMWord soffset_v svlaue_v :: U_MSTORE EVMWord soffset'_v svlaue_v' :: smem'')).
+           exists (eval_common.EvalCommon.update_memory mem (U_MSTORE8 EVMWord soffset_v svlaue_v :: U_MSTORE EVMWord soffset'_v svlaue_v' :: smem'_r')).
+	   split. reflexivity.
+           split. reflexivity.
+           intro w.
+           
+           unfold eval_common.EvalCommon.update_memory.
+           fold eval_common.EvalCommon.update_memory.
+           
+           unfold eval_common.EvalCommon.instantiate_memory_update in E_mo_1_0.
+           rewrite H_eval_soffset in E_mo_1_0.
+           rewrite H_eval_svalue in E_mo_1_0.
+           injection E_mo_1_0 as E_e1.
+           
+           unfold eval_common.EvalCommon.instantiate_memory_update in E_mo_2_0.
+           rewrite H_eval_soffset in E_mo_2_0.
+           rewrite H_eval_svalue in E_mo_2_0.
+           injection E_mo_2_0 as E_e2.
+           
+           rewrite E_updates_1 in H_eval_u_smem'.
+           unfold eval_common.EvalCommon.update_memory in H_eval_u_smem'.
+           fold eval_common.EvalCommon.update_memory in H_eval_u_smem'.
+           injection H_eval_u_smem' as H_eval_u_smem'.
+           
+           rewrite E_updates_2 in H_eval_u_smem'_r.
+           unfold eval_common.EvalCommon.update_memory in H_eval_u_smem'_r.
+           fold eval_common.EvalCommon.update_memory in H_eval_u_smem'_r.
+           injection H_eval_u_smem'_r as H_eval_u_smem'_r.
+           rewrite H_eq_mem1'_mem2'_f in H_eval_u_smem'.
+           rewrite <- H_eval_u_smem'_r in H_eval_u_smem'.
+           
+           rewrite <- E_e1 in H_eval_u_smem'.
+           rewrite <- E_e2 in H_eval_u_smem'.
+           
+           apply mem_eq_when_after_update_eq in H_eval_u_smem'.
+           rewrite H_eval_u_smem'.
+           reflexivity.
+           
+
+        (* MSTORE8 *)
+        ++ simpl in H_valid_smem.
+           destruct H_valid_smem as [ [H_valid_soffset' H_valid_svalue'] H_valid_smem'].
+           destruct (sstack_val_cmp (S (get_maxidx_smap m)) soffset soffset' (get_maxidx_smap m) (get_bindings_smap m) (get_maxidx_smap m) (get_bindings_smap m) instk_height ops) eqn:E_cmp_soffset_soffset'.
+           +++ pose proof (IHsmem' smem_r H_valid_smem' H_basic_mstore_up) as IHsmem'_0.       
+               destruct IHsmem'_0 as [mem1' [mem2' [IHsmem'_0_1 [IHsmem'_0_2 IHsmem'_0_3]]]].
+               unfold safe_sstack_val_cmp_ext_1_d in H_sstack_val_cmp_snd.
+               unfold safe_sstack_val_cmp in H_sstack_val_cmp_snd.
+               pose proof (H_sstack_val_cmp_snd (S (get_maxidx_smap m)) (S (get_maxidx_smap m)) (Nat.le_refl (S (get_maxidx_smap m))) soffset soffset' (get_maxidx_smap m) (get_bindings_smap m) (get_maxidx_smap m) (get_bindings_smap m) instk_height ops H_valid_soffset H_valid_soffset' H_valid_smap H_valid_smap E_cmp_soffset_soffset' stk mem strg ctx H_stk_len) as H_eq_soffset_soffset'.
+               destruct H_eq_soffset_soffset' as [soffset_v [ H_eval_soffset H_eval_soffset']].
+
+               pose proof (two_consecutive_mstore8_updates_same_address soffset soffset' svalue svalue' smem' (get_maxidx_smap m) (get_bindings_smap m) stk mem strg ctx ops soffset_v H_eval_soffset H_eval_soffset') as H_remove_soffset'.
+               rewrite H_remove_soffset'.
+
+               rewrite IHsmem'_0_1.
+               rewrite IHsmem'_0_2.
+
+               exists mem1'.
+               exists mem2'.
+               
+               repeat split; try reflexivity.
+               apply IHsmem'_0_3.
+           +++ rewrite <- H_basic_mstore_up. 
+
+               remember (basic_smemory_updater_remove_mstore8_dups sstack_val_cmp soffset smem' instk_height m ops) as smem'_r.
+               rewrite Heqsmem'_r in *.
+               symmetry in Heqsmem'_r.
+               rewrite Heqsmem'_r.
+               
+               pose proof (IHsmem' smem'_r H_valid_smem' Heqsmem'_r) as IHsmem'_0.
+               destruct IHsmem'_0 as [mem1' [mem2' [H_eval_u_smem' [H_eval_u_smem'_r H_eq_mem1'_mem2']]]].
+               apply functional_extensionality in H_eq_mem1'_mem2' as H_eq_mem1'_mem2'_f.
+
+               pose proof (eval_sstack_val'_succ (S (get_maxidx_smap m)) instk_height soffset stk mem strg ctx (get_maxidx_smap m) (get_bindings_smap m) ops (eq_sym H_stk_len) H_valid_soffset H_valid_smap (gt_Sn_n ((get_maxidx_smap m)))) as H_eval_soffset.
+               destruct H_eval_soffset as [soffset_v H_eval_soffset].
+               
+               pose proof (eval_sstack_val'_succ (S (get_maxidx_smap m)) instk_height soffset' stk mem strg ctx (get_maxidx_smap m) (get_bindings_smap m) ops (eq_sym H_stk_len) H_valid_soffset' H_valid_smap (gt_Sn_n ((get_maxidx_smap m)))) as H_eval_soffset'.
+               destruct H_eval_soffset' as [soffset'_v H_eval_soffset'].
+
+               pose proof (eval_sstack_val'_succ (S (get_maxidx_smap m)) instk_height svalue stk mem strg ctx (get_maxidx_smap m) (get_bindings_smap m) ops (eq_sym H_stk_len) H_valid_svalue H_valid_smap (gt_Sn_n ((get_maxidx_smap m)))) as H_eval_svalue.
+               destruct H_eval_svalue as [svlaue_v H_eval_svalue].
+
+               pose proof (eval_sstack_val'_succ (S (get_maxidx_smap m)) instk_height svalue' stk mem strg ctx (get_maxidx_smap m) (get_bindings_smap m) ops (eq_sym H_stk_len) H_valid_svalue' H_valid_smap (gt_Sn_n ((get_maxidx_smap m)))) as H_eval_svalue'.
+               destruct H_eval_svalue' as [svlaue_v' H_eval_svalue'].
+
+               unfold eval_smemory.
+               unfold map_option.
+               repeat rewrite <- map_option_ho.
+
+               unfold eval_common.EvalCommon.instantiate_memory_update at 1.
+               unfold eval_sstack_val.
+               rewrite H_eval_soffset.
+               rewrite H_eval_svalue.
+
+               unfold eval_common.EvalCommon.instantiate_memory_update at 1.
+               unfold eval_sstack_val.
+               rewrite H_eval_soffset'.
+               rewrite H_eval_svalue'.
+              
+               unfold eval_common.EvalCommon.instantiate_memory_update at 2.
+               rewrite H_eval_soffset.
+               rewrite H_eval_svalue.
+
+               unfold eval_common.EvalCommon.instantiate_memory_update at 2.
+               unfold eval_sstack_val.
+               rewrite H_eval_soffset'.
+               rewrite H_eval_svalue'.
+
+               unfold eval_smemory in H_eval_u_smem'.
+               unfold eval_sstack_val in  H_eval_u_smem'.
+               
+
+               destruct (map_option (eval_common.EvalCommon.instantiate_memory_update (fun sv : sstack_val => eval_sstack_val'  (S (get_maxidx_smap m)) sv stk mem strg ctx (get_maxidx_smap m) (get_bindings_smap m) ops)) (U_MSTORE8 sstack_val soffset svalue :: smem')) as [updates1|] eqn:E_mo_1; try discriminate.
+               pose proof (map_option_split (memory_update sstack_val) (memory_update EVMWord) (eval_common.EvalCommon.instantiate_memory_update (fun sv : sstack_val => eval_sstack_val' (S (get_maxidx_smap m)) sv stk mem strg ctx (get_maxidx_smap m) (get_bindings_smap m) ops)) smem' updates1 (U_MSTORE8 sstack_val soffset svalue) E_mo_1) as E_mo_1_split.
+               destruct E_mo_1_split as [e1 [smem'' [E_updates_1 [E_mo_1_0 E_mo_1_1]]]].
+               rewrite E_mo_1_1.
+
+               unfold eval_smemory in H_eval_u_smem'_r.
+               unfold eval_sstack_val in  H_eval_u_smem'_r.
+               destruct (map_option (eval_common.EvalCommon.instantiate_memory_update (fun sv : sstack_val => eval_sstack_val'  (S (get_maxidx_smap m)) sv stk mem strg ctx (get_maxidx_smap m) (get_bindings_smap m) ops)) (U_MSTORE8 sstack_val soffset svalue :: smem'_r)) as [updates2|] eqn:E_mo_2; try discriminate.
+               pose proof (map_option_split (memory_update sstack_val) (memory_update EVMWord) (eval_common.EvalCommon.instantiate_memory_update (fun sv : sstack_val => eval_sstack_val' (S (get_maxidx_smap m)) sv stk mem strg ctx (get_maxidx_smap m) (get_bindings_smap m) ops)) smem'_r updates2 (U_MSTORE8 sstack_val soffset svalue) E_mo_2) as E_mo_2_split.
+               destruct E_mo_2_split as [e2 [smem'_r' [E_updates_2 [E_mo_2_0 E_mo_2_1]]]].
+               rewrite E_mo_2_1.
+
+               exists (eval_common.EvalCommon.update_memory mem (U_MSTORE8 EVMWord soffset_v svlaue_v :: U_MSTORE8 EVMWord soffset'_v svlaue_v' :: smem'')).
+               exists (eval_common.EvalCommon.update_memory mem (U_MSTORE8 EVMWord soffset_v svlaue_v :: U_MSTORE8 EVMWord soffset'_v svlaue_v' :: smem'_r')).
+	       split. reflexivity.
+               split. reflexivity.
+               intro w.
+               
+               unfold eval_common.EvalCommon.update_memory.
+               fold eval_common.EvalCommon.update_memory.
+
+               unfold eval_common.EvalCommon.instantiate_memory_update in E_mo_1_0.
+               rewrite H_eval_soffset in E_mo_1_0.
+               rewrite H_eval_svalue in E_mo_1_0.
+               injection E_mo_1_0 as E_e1.
+               
+               unfold eval_common.EvalCommon.instantiate_memory_update in E_mo_2_0.
+               rewrite H_eval_soffset in E_mo_2_0.
+               rewrite H_eval_svalue in E_mo_2_0.
+               injection E_mo_2_0 as E_e2.
+
+               rewrite E_updates_1 in H_eval_u_smem'.
+               unfold eval_common.EvalCommon.update_memory in H_eval_u_smem'.
+               fold eval_common.EvalCommon.update_memory in H_eval_u_smem'.
+               injection H_eval_u_smem' as H_eval_u_smem'.
+
+               rewrite E_updates_2 in H_eval_u_smem'_r.
+               unfold eval_common.EvalCommon.update_memory in H_eval_u_smem'_r.
+               fold eval_common.EvalCommon.update_memory in H_eval_u_smem'_r.
+               injection H_eval_u_smem'_r as H_eval_u_smem'_r.
+               rewrite H_eq_mem1'_mem2'_f in H_eval_u_smem'.
+               rewrite <- H_eval_u_smem'_r in H_eval_u_smem'.
+
+               rewrite <- E_e1 in H_eval_u_smem'.
+               rewrite <- E_e2 in H_eval_u_smem'.
+
+               apply mem_eq_when_after_update_eq in H_eval_u_smem'.
+               rewrite H_eval_u_smem'.
+               reflexivity.
+    Qed.
+      
+
+
   Lemma basic_smemory_updater_snd: smemory_updater_ext_snd basic_smemory_updater.
-  Admitted.
+    unfold smemory_updater_ext_snd.
+    intros sstack_val_cmp H_sstack_val_cmp_snd.
+    unfold smemory_updater_snd.
+    split.
+      (* Validity *)
+    + apply basic_smemory_updater_valid.
+      apply H_sstack_val_cmp_snd. 
+    + unfold smemory_updater_correct_res.
+      intros m smem smem' u instk_height ops H_valid_smap H_valid_smem H_valid_u H_basic_smem_updater.
+      intros stk mem strg ctx H_stk_len.
+      unfold basic_smemory_updater in H_basic_smem_updater.
+      destruct u as [soffset svalue|soffset svalue] eqn:E_u.
+      ++ simpl in H_valid_u.
+         destruct H_valid_u as [H_valid_soffset H_valid_svalue].
+         destruct smem' as [|u' smem'']; try discriminate.
+         injection H_basic_smem_updater as H_u' H_smem''.
+         pose proof (basic_smemory_updater_remove_mstore_dups_correct sstack_val_cmp soffset svalue instk_height stk mem strg ctx m ops H_sstack_val_cmp_snd H_stk_len H_valid_soffset H_valid_svalue H_valid_smap smem smem''  H_valid_smem H_smem'') as H_basic_smemory_updater_remove_mstore_dups_correct.
+         destruct H_basic_smemory_updater_remove_mstore_dups_correct as [mem1 [mem2 H_basic_smemory_updater_remove_mstore_dups_correct]].
+         destruct H_basic_smemory_updater_remove_mstore_dups_correct as [H_mem1 [H_mem2 H_eq_mem1_mem2]].
+         rewrite <- H_u'.
+         rewrite H_mem1.
+         rewrite H_mem2.
+         exists mem1.
+         exists mem2.
+         repeat split; try reflexivity.
+         unfold eq_memory.
+         apply H_eq_mem1_mem2.
+      ++ simpl in H_valid_u.
+         destruct H_valid_u as [H_valid_soffset H_valid_svalue].
+         destruct smem' as [|u' smem'']; try discriminate.
+         injection H_basic_smem_updater as H_u' H_smem''.
+         pose proof (basic_smemory_updater_remove_mstore8_dups_correct sstack_val_cmp soffset svalue instk_height stk mem strg ctx m ops H_sstack_val_cmp_snd H_stk_len H_valid_soffset H_valid_svalue H_valid_smap smem smem''  H_valid_smem H_smem'') as H_basic_smemory_updater_remove_mstore8_dups_correct.
+         destruct H_basic_smemory_updater_remove_mstore8_dups_correct as [mem1 [mem2 H_basic_smemory_updater_remove_mstore8_dups_correct]].
+         destruct H_basic_smemory_updater_remove_mstore8_dups_correct as [H_mem1 [H_mem2 H_eq_mem1_mem2]].
+         rewrite <- H_u'.
+         rewrite H_mem1.
+         rewrite H_mem2.
+         exists mem1.
+         exists mem2.
+         repeat split; try reflexivity.
+         unfold eq_memory.
+         apply H_eq_mem1_mem2.
+  Qed.
+
   
 
 End MemoryOpsSolversImplSoundness.
