valid_symbolic_state.v
@@ -783,7 +783,7 @@ Proof.
 Qed.
 
 (* a memory is still valid when extended with a valid update *)
-Lemma valid_smemeory_when_extended_with_valid_update:
+Lemma valid_smemory_when_extended_with_valid_update:
   forall instk_height maxidx u smem,
     valid_smemory_update instk_height maxidx u ->
     valid_smemory instk_height maxidx smem ->
